WIP

bedrock2/src/Examples/bsearch.v
@@ -11,7 +11,7 @@ From bedrock2 Require Import Semantics BasicC64Semantics.
 Local Instance mapok: map.ok mem := SortedListWord.ok (Naive.word 64 eq_refl) _.
 Local Instance wordok: coqutil.Word.Interface.word.ok word := coqutil.Word.Naive.ok _ _.
 Local Instance byteok: coqutil.Word.Interface.word.ok byte := coqutil.Word.Naive.ok _ _.
-Require Import AdmitAxiom.
+Definition admit {T} : T. Admitted.
 
 Goal exists (x4 : list word) (x5 : mem -> Prop), forall M : mem,
     sep (array scalar (word.of_Z 0) (word.of_Z 0) x4) x5 M ->
@@ -19,11 +19,72 @@ Goal exists (x4 : list word) (x5 : mem -> Prop), forall M : mem,
 .
 Proof.
   unshelve (refine (ex_intro _ ?[e1] _); refine (ex_intro _ ?[e2] _); intros M H); cycle -1.
-  1: unshelve epose proof ((match proof_admitted with end : forall n, n = n -> Lift1Prop.iff1
+  1: unshelve epose proof ((admit : forall n, n = n -> Lift1Prop.iff1
        (sep (array scalar (word.of_Z 0) (word.of_Z 0) ?[Goal]) (sep ?[P] ?[Q]))
        (array ?[element] ?[a] ?[aa] ?[xs]))_) as Hrw; cycle -1.
   1: unshelve (let Hrw := open_constr:((Hrw _)) in clear H;
-       epose proof (proj1 (SeparationLogic.Proper_sep_iff1 _ _ Hrw _ _ (RelationClasses.reflexivity _) _) match proof_admitted with end) as XX).
+       epose proof (proj1 (SeparationLogic.Proper_sep_iff1 _ _ Hrw _ _ (RelationClasses.reflexivity _) _) admit) as XX).
   1: destruct M.
-  all: case proof_admitted.
+  all: apply admit.
+  Show Proof.
+(* (ex_intro *)
+(*    (fun x4 : list word => *)
+(*     exists x5 : mem -> Prop, *)
+(*       forall M : mem, *)
+(*       sep (array scalar (word.of_Z 0) (word.of_Z 0) x4) x5 M -> *)
+(*       sep (array scalar (word.of_Z 0) (word.of_Z 0) nil) *)
+(*         (fun _ : mem => False) M) admit *)
+(*    (ex_intro *)
+(*       (fun x5 : mem -> Prop => *)
+(*        forall M : mem, *)
+(*        sep (array scalar (word.of_Z 0) (word.of_Z 0) admit) x5 M -> *)
+(*        sep (array scalar (word.of_Z 0) (word.of_Z 0) nil) *)
+(*          (fun _ : mem => False) M) admit *)
+(*       (fun (M : mem) *)
+(*          (_ : sep (array scalar (word.of_Z 0) (word.of_Z 0) admit) admit M) *)
+(*        => *)
+(*        let Hrw : *)
+(*          admit = admit -> *)
+(*          Lift1Prop.iff1 *)
+(*            (sep (array scalar (word.of_Z 0) (word.of_Z 0) admit) *)
+(*               (sep admit admit)) (array admit admit admit admit) := *)
+(*          admit admit in *)
+(*        let XX : sep (array admit admit admit admit) admit admit := *)
+(*          proj1 *)
+(*            (SeparationLogic.Proper_sep_iff1 *)
+(*               (sep (array scalar (word.of_Z 0) (word.of_Z 0) admit) *)
+(*                  (sep admit admit)) (array admit admit admit admit) *)
+(*               (Hrw *)
+(*                  (match *)
+(*                     M as r *)
+(*                     return *)
+(*                       (sep (array scalar (word.of_Z 0) (word.of_Z 0) admit) *)
+(*                          admit r -> *)
+(*                        (admit = admit -> *)
+(*                         Lift1Prop.iff1 *)
+(*                           (sep *)
+(*                              (array scalar (word.of_Z 0) (word.of_Z 0) admit) *)
+(*                              (sep admit admit)) *)
+(*                           (array admit admit admit admit)) ->  *)
+(*                        admit = admit) *)
+(*                   with *)
+(*                   | {| SortedList.value := value; SortedList._value_ok := *)
+(*                     _value_ok |} => *)
+(*                       fun *)
+(*                         (_ : sep *)
+(*                                (array scalar (word.of_Z 0)  *)
+(*                                   (word.of_Z 0) admit) admit *)
+(*                                {| *)
+(*                                SortedList.value := value; *)
+(*                                SortedList._value_ok := _value_ok |}) *)
+(*                         (_ : admit = admit -> *)
+(*                              Lift1Prop.iff1 *)
+(*                                (sep *)
+(*                                   (array scalar (word.of_Z 0)  *)
+(*                                      (word.of_Z 0) admit)  *)
+(*                                   (sep admit admit)) *)
+(*                                (array admit admit admit admit)) => admit *)
+(*                   end H Hrw)) admit admit (RelationClasses.reflexivity admit) *)
+(*               admit) admit in *)
+(*        admit))) *)
 Qed. (* Error: No such section variable or assumption: H9. *)
